src/Std/Data/Iterators/Producers/Monadic/Array.lean
@@ -7,6 +7,7 @@ module
 
 prelude
 public import Init.Data.Iterators.Consumers
+public import Init.Data.Nat.MinMax
 import Init.Omega
 
 @[expose] public section
@@ -14,7 +15,8 @@ import Init.Omega
 /-!
 # Array iterator
 
-This module provides an iterator for arrays that is accessible via `Array.iterM`.
+This module provides forward and reverse iterators for arrays that are accessible via
+`Array.iterM` and `Array.iterRevM`.
 -/
 
 namespace Std.Iterators.Types
@@ -22,7 +24,7 @@ namespace Std.Iterators.Types
 variable {α : Type w} {m : Type w → Type w'}
 
 /--
-The underlying state of a list iterator. Its contents are internal and should
+The underlying state of an array iterator. Its contents are internal and should
 not be used by downstream users of the library.
 -/
 @[unbox, ext]
@@ -113,6 +115,107 @@ instance ArrayIterator.instFinite [Pure m] : Finite (ArrayIterator α) m := by
 
 @[always_inline, inline]
 instance ArrayIterator.instIteratorLoop {α : Type w} [Monad m] {n : Type x → Type x'} [Monad n] :
+    IteratorLoop (ArrayIterator α) m n :=
+  .defaultImplementation
+
+/--
+The underlying state of a reverse array iterator. Its contents are internal and should
+not be used by downstream users of the library.
+-/
+@[unbox, ext]
+structure ArrayRevIterator (α : Type w) where
+  /-- Internal implementation detail of the iterator library. -/
+  array : Array α
+  /-- Internal implementation detail of the iterator library. -/
+  pos : Nat
+  /-- Internal implementation detail of the iterator library. -/
+  upper_bound : pos ≤ array.size
+
+theorem ArrayRevIterator.exists_iff {α : Type w} {P : ArrayRevIterator α → Prop} :
+    (∃ s, P s) ↔ ∃ array pos upper_bound, P ⟨array, pos, upper_bound⟩ := by
+  constructor
+  · rintro ⟨⟨array, pos, upper_bound⟩, h⟩
+    exact ⟨array, pos, upper_bound, h⟩
+  · rintro ⟨array, pos, upper_bound, h⟩
+    exact ⟨⟨array, pos, upper_bound⟩, h⟩
+
+/--
+Returns a finite monadic reverse iterator for the given array starting at the given index.
+The iterator yields the elements of the array in reverse order and then terminates.
+
+The pure version of this iterator is `Array.iterRevFromIdx`.
+
+**Termination properties:**
+
+* `Finite` instance: always
+* `Productive` instance: always
+-/
+@[always_inline, inline, match_pattern]
+def _root_.Array.iterRevFromIdxM {α : Type w} (array : Array α) (m : Type w → Type w') (pos : Nat)
+    [Pure m] :
+    IterM (α := ArrayRevIterator α) m α :=
+  ⟨{ array := array, pos := (pos + 1).min array.size, upper_bound := Nat.min_le_right _ _ }⟩
+
+/--
+Returns a finite monadic reverse iterator for the given array.
+The iterator yields the elements of the array in reverse order and then terminates. There are
+no side effects.
+
+The pure version of this iterator is `Array.iterRev`.
+
+**Termination properties:**
+
+* `Finite` instance: always
+* `Productive` instance: always
+-/
+@[always_inline, inline]
+def _root_.Array.iterRevM {α : Type w} (array : Array α) (m : Type w → Type w') [Pure m] :
+    IterM (α := ArrayRevIterator α) m α :=
+  array.iterRevFromIdxM m array.size
+
+@[always_inline, inline]
+instance ArrayRevIterator.instIterator {α : Type w} [Pure m] :
+    Iterator (ArrayRevIterator α) m α where
+  IsPlausibleStep it
+    | .yield it' out => it.internalState.array = it'.internalState.array ∧
+      ∃ _ : it'.internalState.pos + 1 = it.internalState.pos ∧
+      it.internalState.pos ≤ it.internalState.array.size,
+      have h : it'.internalState.pos < it.internalState.array.size := by omega
+      it.internalState.array[it'.internalState.pos] = out
+    | .skip _ => False
+    | .done => it.internalState.pos = 0
+  step it := pure <| .deflate <| if h : 0 < it.internalState.pos then
+        let ⟨⟨array, pos, h'⟩⟩ := it
+        have h'' : pos - 1 < array.size := by simp at h; omega
+        .yield
+          ⟨⟨array, pos - 1, by omega⟩⟩
+          array[pos - 1]
+          ⟨rfl, ⟨by simp at h ⊢ ; omega, h'⟩, rfl⟩
+      else
+        .done (by simp; omega)
+
+private def ArrayRevIterator.instFinitenessRelation [Pure m] :
+    FinitenessRelation (ArrayIterator α) m where
+  Rel := InvImage WellFoundedRelation.rel
+      (fun it => it.internalState.array.size - it.internalState.pos)
+  wf := InvImage.wf _ WellFoundedRelation.wf
+  subrelation {it it'} h := by
+    simp_wf
+    obtain ⟨step, h, h'⟩ := h
+    cases step
+    · cases h
+      obtain ⟨h, h', h'', rfl⟩ := h'
+      rw [h] at h''
+      rw [h, h']
+      omega
+    · cases h'
+    · cases h
+
+instance ArrayRevIterator.instFinite [Pure m] : Finite (ArrayIterator α) m := by
+  exact Finite.of_finitenessRelation ArrayIterator.instFinitenessRelation
+
+@[always_inline, inline]
+instance ArrayRevIterator.instIteratorLoop {α : Type w} [Monad m] {n : Type x → Type x'} [Monad n] :
     IteratorLoop (ArrayIterator α) m n :=
   .defaultImplementation
 
